\begin{minipage}{0.485\textwidth}
    \enteteInterro{Le 19 septembre 2014}{1}{A}

    Calculer :
    \begin{enumerate}
        \item
            \( (-1)+(-7)=\ldots\)
        \item
            \( (-4)\times 4=\ldots\)
        \item
            \( (+5)-(+7)=\ldots\)
        \item
            \( \dfrac{ 9 }{ -3 }=\ldots\)
        \item
            \( (-12)\times (-2)=\ldots\)
    \end{enumerate}

\end{minipage}
\begin{minipage}{0.485\textwidth}
    \enteteInterro{Le 19 septembre 2014}{1}{B}

    Calculer :
    \begin{enumerate}
        \item
            \( (+5)\times (-12)=\ldots\)
        \item
            \( \dfrac{ 12 }{ -4 }=\ldots\)
        \item
            \( (-4)\times (-5)=\ldots\)
        \item
            \( (+10)-(+14)=\ldots\)
        \item
            \( (-9)+(-3)=\ldots\)
    \end{enumerate}

\end{minipage}
